assembly/Lens.v
@@ -9,7 +9,7 @@ Require Export Coq.Setoids.Setoid.
 Require Import Assembly.Convenience.
 Require Import Assembly.Dec.
 
-Class Proj (S: Type) (X: Type) :=
+Class Lens (S: Type) (X: Type) :=
 {
   proj: S -> X;
   update: S -> X -> S;
@@ -23,12 +23,12 @@ Create HintDb proj discriminated.
 Hint Rewrite @proj_update using (typeclasses eauto) : proj.
 Hint Rewrite @update_proj using (typeclasses eauto) : proj.
 Hint Rewrite @update_update using (typeclasses eauto) : proj.
-Ltac proj_rewrite1 := rewrite_strat (outermost (hints proj)).
-Ltac proj_rewrite := repeat proj_rewrite1.
+Ltac lens_rewrite1 := rewrite_strat (outermost (hints proj)).
+Ltac lens_rewrite := repeat lens_rewrite1.
 
 Class Independent {S: Type}
-      {X: Type} (PX: Proj S X)
-      {Y: Type} (PY: Proj S Y) : Prop :=
+      {X: Type} (LX: Lens S X)
+      {Y: Type} (LY: Lens S Y) : Prop :=
 {
   projY_updateX (s: S) (x: X) : proj (update s x) = proj s :> Y;
   projX_updateY (s: S) (y: Y) : proj (update s y) = proj s :> X;
@@ -53,35 +53,35 @@ Section product_section.
   (* Since this instance is in a section and not marked global,
      it is removed from the instance database below. *)
 
-  Program Instance proj_fst : Proj (X * Y) X :=
+  Program Instance lens_fst : Lens (X * Y) X :=
   {
     proj := fst;
     update s x := (x, snd s);
   }.
 
-  Program Instance proj_snd : Proj (X * Y) Y :=
+  Program Instance lens_snd : Lens (X * Y) Y :=
   {
     proj := snd;
     update s y := (fst s, y);
   }.
 
-  Program Instance independent_projs : Independent proj_fst proj_snd.
+  Program Instance independent_projs : Independent lens_fst lens_snd.
 
-  Context {S} (PX: Proj S X) (PY: Proj S Y) {Hd: Independent PX PY}.
+  Context {S} (LX: Lens S X) (LY: Lens S Y) {Hd: Independent LX LY}.
 
   #[refine]
-  Instance proj_prod : Proj S (X * Y) :=
+  Instance lens_prod : Lens S (X * Y) :=
   {
     proj s := (proj s, proj s);
     update s pair := update (update s (fst pair)) (snd pair);
   }.
   Proof.
-    all: idestructs; now repeat (independent_rewrite1 || proj_rewrite || simpl).
+    all: idestructs; now repeat (independent_rewrite1 || lens_rewrite || simpl).
   Defined.
 
-  Context Z (PZ: Proj S Z) (Hdx: Independent PX PZ) (Hdy: Independent PY PZ).
+  Context Z (PZ: Lens S Z) (Hdx: Independent LX PZ) (Hdy: Independent LY PZ).
 
-  Global Instance independent_prod : Independent proj_prod PZ.
+  Global Instance independent_prod : Independent lens_prod PZ.
   Proof using Hdx Hdy.
     split.
     - intros s [x y]. simpl.
@@ -93,11 +93,11 @@ Section product_section.
   (** Beware: We do not make this global sine together with
       [independent_commute] it can send [typeclasses eauto]
       into an infinite loop. *)
-  Instance independent_symm : Independent PY PX.
+  Instance independent_symm : Independent LY LX.
   Proof using Hd.
     split; intros; now independent_rewrite.
   Qed.
 
 End product_section.
 
-(** The projections from a record type have the same property. *)
+(** The projections from a record type have the same property, cf. Concrete.v. *)
